theories/logrel/contexts.v
@@ -1,0 +1,243 @@
+(** This file contains definitions related to type ctxironments. The following
+relations on ctxironments are defined:
+
+- [ctx_ltyped Γ vs]: This relation indicates that the value map [vs] contains a
+  value for each type in the semantic type ctxironment [Γ].
+- [ctx_split Γ Γ1 Γ2]: The semantic type ctxironment [Γ] can be split into
+  (semantically disjoint) [Γ1] and [Γ2].
+- [ctx_copy Γ Γ']: [Γ'] is a copyable sub-ctxironment of [Γ].
+
+In addition, some lemmas/rules about these definitions are proved, corresponding
+to the syntactic typing rules that are typically found in substructural type
+systems. *)
+From iris.algebra Require Export list.
+From iris.bi.lib Require Import core.
+From iris.proofmode Require Import tactics.
+From actris.logrel Require Export term_types subtyping_rules.
+
+Inductive ctx_item Σ := CtxItem {
+  ctx_item_name : string;
+  ctx_item_type : ltty Σ;
+}.
+Add Printing Constructor ctx_item.
+Arguments CtxItem {_} _ _.
+Arguments ctx_item_name {_} _.
+Arguments ctx_item_type {_} _.
+Instance: Params (@CtxItem) 2 := {}.
+Instance: Params (@ctx_item_type) 1 := {}.
+
+Section ctx_item_ofe.
+  Context {Σ : gFunctors}.
+  Instance ctx_item_equiv : Equiv (ctx_item Σ) := λ xA1 xA2,
+    ctx_item_name xA1 = ctx_item_name xA2 ∧ ctx_item_type xA1 ≡ ctx_item_type xA2.
+  Instance ctx_item_dist : Dist (ctx_item Σ) := λ n xA1 xA2,
+    ctx_item_name xA1 = ctx_item_name xA2 ∧ ctx_item_type xA1 ≡{n}≡ ctx_item_type xA2.
+  Lemma ctx_item_ofe_mixin : OfeMixin (ctx_item Σ).
+  Proof.
+    by apply (iso_ofe_mixin (A:=prodO (leibnizO string) (lttyO Σ))
+      (λ xA, (ctx_item_name xA, ctx_item_type xA))).
+  Qed.
+  Canonical Structure ctx_itemO := OfeT (ctx_item Σ) ctx_item_ofe_mixin.
+  Global Instance ctx_item_type_ne : NonExpansive (@ctx_item_type Σ).
+  Proof. by intros n ?? [??]. Qed.
+  Global Instance ctx_item_type_proper : Proper ((≡) ==> (≡)) (@ctx_item_type Σ).
+  Proof. by intros ?? [??]. Qed.
+End ctx_item_ofe.
+
+Notation ctx Σ := (list (ctx_item Σ)).
+
+Definition ctx_filter_eq {Σ} (x : binder) : ctx Σ → ctx Σ :=
+  filter (λ xA, x = BNamed (ctx_item_name xA)).
+Definition ctx_filter_ne {Σ} (x : binder) : ctx Σ → ctx Σ :=
+  filter (λ xA, x ≠ BNamed (ctx_item_name xA)).
+
+Arguments ctx_filter_eq _ !_ !_ / : simpl nomatch.
+Arguments ctx_filter_ne _ !_ !_ / : simpl nomatch.
+(** TODO: Move to std++, together with some lemmas about filter that can be
+factored out. *)
+Arguments filter _ _ _ _ _ !_ / : simpl nomatch.
+
+Instance ctx_lookup {Σ} : Lookup string (ltty Σ) (ctx Σ) := λ x Γ,
+  match ctx_filter_eq x Γ with
+  | [CtxItem _ A] => Some A
+  | _ => None
+  end.
+
+Definition ctx_cons {Σ} (b : binder) (A : ltty Σ) (Γ : ctx Σ) : ctx Σ :=
+  if b is BNamed x then CtxItem x A :: ctx_filter_ne x Γ else Γ.
+
+Definition ctx_ltyped {Σ} (vs : gmap string val) (Γ : ctx Σ) : iProp Σ :=
+  ([∗ list] iA ∈ Γ, ∃ v,
+    ⌜vs !! ctx_item_name iA = Some v⌝ ∗ ltty_car (ctx_item_type iA) v)%I.
+Instance: Params (@ctx_ltyped) 2 := {}.
+
+Definition ctx_le {Σ} (Γ1 Γ2 : ctx Σ) : iProp Σ :=
+  tc_opaque (■ ∀ vs, ctx_ltyped vs Γ1 -∗ ctx_ltyped vs Γ2)%I.
+Instance: Params (@ctx_le) 1 := {}.
+Infix "<ctx:" := ctx_le (at level 70) : bi_scope.
+Notation "Γ1 <ctx: Γ2" := (⊢ Γ1 <ctx: Γ2) (at level 70) : type_scope.
+
+Section ctx.
+  Context {Σ : gFunctors}.
+  Implicit Types A : ltty Σ.
+  Implicit Types Γ : ctx Σ.
+
+  (** ctx_filter *)
+  Lemma ctx_filter_eq_perm Γ x : Γ ≡ₚ ctx_filter_eq x Γ ++ ctx_filter_ne x Γ.
+  Proof.
+    rewrite /ctx_filter_eq /ctx_filter_ne.
+    induction Γ as [|[y A] Γ IH]; simpl; [done|].
+    rewrite filter_cons. case_decide.
+    - rewrite filter_cons_False /=; last naive_solver. by rewrite -IH.
+    - rewrite filter_cons_True /=; last naive_solver.
+      by rewrite -Permutation_middle -IH.
+  Qed.
+
+  Lemma ctx_filter_ne_anon Γ : ctx_filter_ne BAnon Γ = Γ.
+  Proof. induction Γ as [|[y A] Γ IH]; by f_equal/=. Qed.
+
+  Lemma elem_of_ctx_filter_ne Γ x y B :
+    CtxItem y B ∈ ctx_filter_ne x Γ → x ≠ y.
+  Proof. intros ?%elem_of_list_filter. naive_solver. Qed.
+
+  Lemma ctx_filter_ne_cons Γ (x : string) A :
+    ctx_filter_ne x (CtxItem x A :: Γ) = ctx_filter_ne x Γ.
+  Proof. rewrite /ctx_filter_ne filter_cons_False; naive_solver. Qed.
+  Lemma ctx_filter_ne_cons_ne Γ x y A :
+    x ≠ BNamed y →
+    ctx_filter_ne x (CtxItem y A :: Γ) = CtxItem y A :: ctx_filter_ne x Γ.
+  Proof. intros. rewrite /ctx_filter_ne filter_cons_True; naive_solver. Qed.
+
+  Lemma ctx_lookup_perm Γ x A:
+    Γ !! x = Some A →
+    Γ ≡ₚ CtxItem x A :: ctx_filter_ne x Γ.
+  Proof.
+    rewrite /lookup /ctx_lookup=> ?.
+    destruct (ctx_filter_eq x Γ) as [|[x' ?] [|??]] eqn:Hx; simplify_eq/=.
+    assert (CtxItem x' A ∈ ctx_filter_eq x Γ)
+      as [? _]%elem_of_list_filter; simplify_eq/=.
+    { rewrite Hx. set_solver. }
+    by rewrite {1}(ctx_filter_eq_perm Γ x') Hx.
+  Qed.
+
+  (** ctx typing *)
+  Global Instance ctx_ltyped_Permutation vs :
+    Proper ((≡ₚ) ==> (⊣⊢)) (@ctx_ltyped Σ vs).	
+  Proof. intros Γ Γ' HΓ. by rewrite /ctx_ltyped HΓ. Qed.
+  Global Instance ctx_ltyped_ne vs : NonExpansive (@ctx_ltyped Σ vs).
+  Proof.
+    intros n Γ Γ' HΓ. rewrite /ctx_ltyped.
+    apply big_opL_gen_proper_2; [done|apply _|]. intros k.
+    assert (Γ !! k ≡{n}≡ Γ' !! k) as HΓk by (by rewrite HΓ).
+    case: HΓk=> // -[x1 A1] [x2 A2] [/= -> ?]. by repeat f_equiv.
+  Qed.
+  Global Instance ctx_ltyped_proper vs : Proper ((≡) ==> (≡)) (@ctx_ltyped Σ vs).
+  Proof. apply (ne_proper _). Qed.
+
+  Lemma ctx_ltyped_nil vs : ⊢@{iPropI Σ} ctx_ltyped vs [].
+  Proof. done. Qed.
+
+  Lemma ctx_ltyped_app Γ1 Γ2 vs :
+    ctx_ltyped vs (Γ1 ++ Γ2) ⊣⊢ ctx_ltyped vs Γ1 ∗ ctx_ltyped vs Γ2.
+  Proof. apply big_opL_app. Qed.
+
+  Lemma ctx_ltyped_cons Γ vs x A : 
+    ctx_ltyped vs (CtxItem x A :: Γ) ⊣⊢ ∃ v,
+    ⌜vs !! x = Some v⌝ ∗ ltty_car A v ∗ ctx_ltyped vs Γ.
+  Proof.
+    iSplit; [by iIntros "[HA $]"|].
+    iDestruct 1 as (v ?) "[HA $]"; eauto.
+  Qed.
+
+  Lemma ctx_ltyped_insert Γ vs x A v :
+    ltty_car A v -∗
+    ctx_ltyped vs (ctx_filter_ne x Γ) -∗
+    ctx_ltyped (binder_insert x v vs) (ctx_cons x A Γ).
+  Proof.
+    iIntros "HA HΓ".
+    destruct x as [|x]; simpl; [rewrite ctx_filter_ne_anon; auto|].
+    iApply ctx_ltyped_cons. iExists _; iSplit; [by rewrite lookup_insert|].
+    iFrame "HA". iApply (big_sepL_impl with "HΓ").
+    iIntros "!>" (k [j B] ?%elem_of_list_lookup_2%elem_of_ctx_filter_ne).
+    iDestruct 1 as (w ?) "HB". iExists w. iIntros "{$HB} !%".
+    apply lookup_insert_Some; naive_solver.
+  Qed.
+
+  Lemma ctx_ltyped_insert' Γ vs x A v :
+    ltty_car A v -∗
+    ctx_ltyped vs Γ -∗
+    ctx_ltyped (binder_insert x v vs) (ctx_cons x A Γ).
+  Proof.
+    rewrite {1}(ctx_filter_eq_perm Γ x) ctx_ltyped_app.
+    iIntros "HA [_ HΓ]". by iApply (ctx_ltyped_insert with "HA").
+  Qed.
+
+  Lemma ctx_ltyped_delete Γ x v vs :
+    ctx_ltyped (binder_insert x v vs) Γ -∗
+    ctx_ltyped vs (ctx_filter_ne x Γ).
+  Proof.
+    rewrite {1}(ctx_filter_eq_perm Γ x) ctx_ltyped_app. iIntros "[_ HΓ]".
+    iApply (big_sepL_impl with "HΓ").
+    iIntros "!>" (k [j B] ?%elem_of_list_lookup_2%elem_of_ctx_filter_ne).
+    iDestruct 1 as (w Hx) "HB". simpl in *. iExists w. iIntros "{$HB} !%".
+    destruct x as [|x]; simplify_eq/=; auto.
+    revert Hx. rewrite lookup_insert_Some. naive_solver.
+  Qed.
+
+  (** Ctxironment subtyping *)
+  Global Instance ctx_le_plain Γ1 Γ2 : Plain (Γ1 <ctx: Γ2).
+  Proof. rewrite /ctx_le /=. apply _. Qed.
+
+  Global Instance ctx_le_Permutation : Proper ((≡ₚ) ==> (≡ₚ) ==> (≡)) (@ctx_le Σ).
+  Proof.
+    intros Γ1 Γ1' HΓ1 Γ2 Γ2' HΓ2. rewrite /ctx_le /=.
+    setoid_rewrite HΓ1; by setoid_rewrite HΓ2.
+  Qed.
+  Global Instance ctx_le_ne : NonExpansive2 (@ctx_le Σ).
+  Proof. solve_proper. Qed.
+  Global Instance ctx_le_proper : Proper ((≡) ==> (≡) ==> (≡)) (@ctx_le Σ).
+  Proof. apply (ne_proper_2 _). Qed.
+
+  Lemma ctx_le_refl Γ : Γ <ctx: Γ.
+  Proof. iIntros (vs); auto. Qed.
+  Lemma ctx_le_trans Γ1 Γ2 Γ3 : Γ1 <ctx: Γ2 -∗ Γ2 <ctx: Γ3 -∗ Γ1 <ctx: Γ3.
+  Proof.
+    rewrite /ctx_le /=.
+    iIntros "#H1 #H2 !>" (vs) "Hvs". iApply "H2". by iApply "H1".
+  Qed.
+  Lemma ctx_le_nil Γ : Γ <ctx: [].
+  Proof. iIntros (vs) "!> _". iApply ctx_ltyped_nil. Qed.
+  Lemma ctx_le_cons x Γ1 Γ2 A1 A2 :
+    A1 <: A2 -∗ Γ1 <ctx: Γ2 -∗ CtxItem x A1 :: Γ1 <ctx: CtxItem x A2 :: Γ2.
+  Proof.
+    rewrite /ctx_le /=. iIntros "#H #H' !>" (vs) "Hvs".
+    iDestruct (ctx_ltyped_cons with "Hvs") as (v ?) "[Hv Hvs]".
+    iApply ctx_ltyped_cons. iExists _; iSplit; [done|].
+    iSplitL "Hv"; [by iApply "H"|by iApply "H'"].
+  Qed.
+  Lemma ctx_le_app Γ1 Γ2 Γ1' Γ2' :
+    Γ1 <ctx: Γ2 -∗ Γ1' <ctx: Γ2' -∗ Γ1 ++ Γ1' <ctx: Γ2 ++ Γ2'.
+  Proof.
+    rewrite /ctx_le /=. iIntros "#H #H' !>" (vs) "Hvs".
+    iDestruct (ctx_ltyped_app with "Hvs") as "[Hvs1 Hvs2]".
+    iApply ctx_ltyped_app. iSplitL "Hvs1"; [by iApply "H"|by iApply "H'"].
+  Qed.
+  Lemma ctx_le_copy x A :
+    [CtxItem x A] <ctx: [CtxItem x A; CtxItem x (copy- A)].
+  Proof.
+    iIntros "!>" (vs) "Hvs".
+    iDestruct (ctx_ltyped_cons with "Hvs") as (v ?) "[HA _]".
+    iAssert (ltty_car (copy- A) v)%lty as "#HAm"; [by iApply coreP_intro|].
+    iApply ctx_ltyped_cons. iExists _; iSplit; [done|]. iFrame "HA".
+    iApply ctx_ltyped_cons. iExists _; iSplit; [done|]. iFrame "HAm".
+    iApply ctx_ltyped_nil.
+  Qed.
+  Lemma ctx_le_copyable x A :
+    lty_copyable A -∗
+    [CtxItem x A] <ctx: [CtxItem x A; CtxItem x A].
+  Proof.
+    iIntros "#H". iApply ctx_le_trans; [iApply ctx_le_copy|].
+    iApply ctx_le_cons; [iApply lty_le_refl|].
+    iApply ctx_le_cons; [by iApply lty_le_copy_inv_elim_copyable|iApply ctx_le_nil].
+  Qed.
+End ctx.
