theories/logrel/examples/pair.v
@@ -13,7 +13,7 @@ From iris.proofmode Require Import tactics.
 Definition prog : expr := λ: "c", (recv "c", recv "c").
 
 Lemma prog_typed `{heapG Σ, chanG Σ} :
-  ⊢ [] ⊨ prog : chan (<??> TY lty_int; <??> TY lty_int; END) ⊸ lty_int * lty_int.
+  [] ⊨ prog : chan (<??> TY lty_int; <??> TY lty_int; END) ⊸ lty_int * lty_int.
 Proof.
   iApply (ltyped_lam []); simpl. iApply ltyped_post_nil.
   iApply ltyped_pair; [by iApply ltyped_recv|by iApply ltyped_recv].
