theories/logrel/lib/par_start.v
@@ -10,16 +10,16 @@ Definition par_start : expr := λ: "e1" "e2",
   ("e1" "c1") ||| ("e2" "c2").
 
 Lemma ltyped_par_start `{!heapG Σ, !chanG Σ, !spawnG Σ} Γ S A B :
-  ⊢ Γ ⊨ par_start : (chan S ⊸ A) ⊸ (chan (lty_dual S) ⊸ B) ⊸ A * B.
+  Γ ⊨ par_start : (chan S ⊸ A) ⊸ (chan (lty_dual S) ⊸ B) ⊸ A * B.
 Proof.
-  iApply (ltyped_lam []); iApply (ltyped_lam [EnvItem "e1" _] [] "e2"); simpl.
+  iApply (ltyped_lam []); iApply (ltyped_lam [CtxItem "e1" _] [] "e2"); simpl.
   iApply ltyped_post_nil. iApply ltyped_let.
   { iApply ltyped_app; [iApply ltyped_unit|iApply (ltyped_new_chan _ S)]. }
   iApply ltyped_let; [by iApply ltyped_fst|]; simpl.
   iApply ltyped_let; [by iApply ltyped_snd|]; simpl.
-  rewrite !(Permutation_swap (EnvItem "c1" _))
-    !(Permutation_swap (EnvItem "e1" _)).
-  iApply (ltyped_par [EnvItem "e1" _; EnvItem "c1" _]).
+  rewrite !(Permutation_swap (CtxItem "c1" _))
+    !(Permutation_swap (CtxItem "e1" _)).
+  iApply (ltyped_par [CtxItem "e1" _; CtxItem "c1" _]).
   - iApply ltyped_app; by iApply ltyped_var.
   - iApply ltyped_app; by iApply ltyped_var.
 Qed.
