papers/CPP21.md
@@ -1,4 +1,4 @@
-## Differences
+# Differences between the paper and the mechanisation
 
 - The semantic encoding of ground types use existential quantification in the
   mechanization (e.g., `λ w. ∃ (x:Z), w = int`, while the paper uses set
@@ -14,16 +14,19 @@
 - The mechanisation employs a typing judgement for values (`ltyped_val`),
   for technical reasons. More details on this is found in
   [theories/logrel/term_typing_judgment.v](../theories/logrel/term_typing_judgment.v)
-## Examples
+
+# Examples
 
 - The parallel receive example in Section 4 can be found in
   [theories/logrel/examples/par_recv.v](../theories/logrel/examples/par_recv.v):
-  This program performs two ``racy'' parallel receives on the same channel from
+  This program performs two "racy" parallel receives on the same channel from
   two different threads, using locks to allow the channel to be shared.
 - The parallel compute client example in Section 4 can be found in
   [theories/logrel/examples/compute_client_list.v](../theories/logrel/examples/compute_client_list.v):
   This program sends computation requests and receives their results in parallel,
   analogous to the producer-consumer pattern. It uses a lock to share the channel
   and a shared counter, that keeps track of the number of computations in transit.
-  The computation service can be found in [theories/logrel/examples/compute_service.v](../theories/logrel/examples/compute_service.v). The definition of the list type
-  and the weakest precondition for `llength` can be found in [theories/logrel/lib/list.v](../theories/logrel/lib/list.v)
+  The computation service can be found in
+  [theories/logrel/examples/compute_service.v](../theories/logrel/examples/compute_service.v).
+  The definition of the list type and the weakest precondition for `llength`
+  can be found in [theories/logrel/lib/list.v](../theories/logrel/lib/list.v)
